src/VmSemantics.v
@@ -124,12 +124,12 @@ Proof.
     assert (
         StVM.st_trace
           (snd (copland_compile t1 {| st_ev := (splitEv_l s e);
-                                      st_trace := m ++ (k ++ [Term_Defs.split n p]);
+                                      st_trace := m ++ (k ++ [cvm_split n p]);
                                       st_pl := p |})) =
          m ++
          StVM.st_trace
          (snd (copland_compile t1 {| st_ev := (splitEv_l s e);
-                                     st_trace := k ++ [Term_Defs.split n p];
+                                     st_trace := k ++ [cvm_split n p];
                                      st_pl := p |}))).
     {
       rewrite <- app_assoc in *.
@@ -157,8 +157,8 @@ Proof.
     subst.
     tauto.
 
-  -
-        annogo.
+  - (* abpar case *)
+    annogo.
         
     do_wf_pieces.
     df.
@@ -173,17 +173,17 @@ Proof.
 
     assert (
         StVM.st_trace
-          (snd (copland_compile t1 {| st_ev := (splitEv_l s e);
-                                      st_trace := m ++ (k ++ [Term_Defs.split n p]);
+          (snd (copland_compile t {| st_ev := (splitEv_l s e);
+                                      st_trace := m ++ (k ++ [cvm_splitp n l p a (get_et (splitEv_r s e))]);
                                       st_pl := p |})) =
          m ++
          StVM.st_trace
-         (snd (copland_compile t1 {| st_ev := (splitEv_l s e);
-                                     st_trace := k ++ [Term_Defs.split n p];
+         (snd (copland_compile t {| st_ev := (splitEv_l s e);
+                                     st_trace := k ++ [cvm_splitp n l p a (get_et (splitEv_r s e))];
                                      st_pl := p |}))).
     {
       rewrite <- app_assoc in *.
-      eapply IHt1; eauto.
+      eapply IHt; eauto.
     }
     subst'.
     df.
@@ -191,6 +191,9 @@ Proof.
     subst'.
     df.  
     subst.
+    tauto.
+
+    (*
 
     assert (
         StVM.st_trace (snd (copland_compile t2{| st_ev := (splitEv_r s e);
@@ -203,8 +206,10 @@ Proof.
     eapply IHt2; eauto.
     subst'.
     df.
-    subst.
-    tauto.
+    subst. 
+    tauto. 
+     *)
+    
 Defined.
 
 (* Instance of st_trace_cumul' where k=[] *)
@@ -279,8 +284,8 @@ Ltac do_suffix name :=
   end.
 
 Lemma alseq_decomp_gen : forall r t1' t2' e e'' p p'' init_tr tr,
-    well_formed_r (alseq r t1' t2') ->
-    copland_compile (alseq r t1' t2') {| st_ev := e; st_trace := init_tr; st_pl := p |} =
+    well_formed_r (alseq_par r t1' t2') ->
+    copland_compile (alseq_par r t1' t2') {| st_ev := e; st_trace := init_tr; st_pl := p |} =
     (Some tt, {| st_ev := e''; st_trace := tr; st_pl := p'' |}) ->
 
     exists e' tr' p',
@@ -309,8 +314,8 @@ Proof.
 Defined.
 
 Lemma alseq_decomp : forall r t1' t2' e e'' p p'' tr,
-    well_formed_r (alseq r t1' t2') ->
-    copland_compile (alseq r t1' t2') {| st_ev := e; st_trace := []; st_pl := p |} =
+    well_formed_r (alseq_par r t1' t2') ->
+    copland_compile (alseq_par r t1' t2') {| st_ev := e; st_trace := []; st_pl := p |} =
     (Some tt, {| st_ev := e''; st_trace := tr; st_pl := p'' |}) ->
 
     exists e' tr' p',
@@ -437,10 +442,53 @@ Proof.
   ff.
 Defined.
 
+Lemma aeval_anno: forall a i n e0,
+    (aeval (snd (anno (unanno a) i)) n e0 = aeval a n e0).
+Proof.
+  intros.
+  generalizeEverythingElse a.
+  induction a; intros.
+  -
+    ff.
+  -
+    ff.
+    eauto.
+    simpl.
+    erewrite <- IHa.
+    rewrite Heqp.
+    simpl.
+    tauto.
+  -
+    ff.
+    erewrite <- IHa1.
+    erewrite <- IHa2.
+    rewrite Heqp0.
+    rewrite Heqp.
+    simpl.
+    tauto.
+  -
+    ff.
+    erewrite <- IHa1.
+    erewrite <- IHa2.
+    rewrite Heqp0.
+    rewrite Heqp.
+    simpl.
+    tauto.
+  -
+    ff.
+    erewrite <- IHa1.
+    erewrite <- IHa2.
+    rewrite Heqp0.
+    rewrite Heqp.
+    simpl.
+    tauto.
+Defined.
+
+
 Lemma cvm_refines_lts_evidence' : forall t tr tr' e e' p p',
     well_formed_r t ->
     copland_compile t (mk_st e tr p) = (Some tt, (mk_st e' tr' p')) ->
-    get_et e' = (Term_Defs.eval (unanno t) p (get_et e)).
+    get_et e' = (Term_Defs.eval (unanno (unannoPar t)) p (get_et e)).
 
 Proof.
   induction t; intros.
@@ -455,10 +503,21 @@ Proof.
     repeat df. 
     annogo.
     do_wf_pieces.
+    destruct e.
+    ff.
+    erewrite eval_aeval.
+    simpl.
+        
+    rewrite aeval_anno.
+    eapply remote_Evidence_Type_Axiom.
+
+    (*
     eapply IHt.
-    eassumption.  
+    eassumption.
     eapply copland_compile_at.
     eassumption.
+     *)
+    
 
   - (* alseq case *)
     do_wf_pieces.
@@ -505,7 +564,7 @@ Proof.
       assert (e3 = get_et (evc e2 e3)) by tauto.
       jkjke.
 
-      assert (get_et (evc e0 e1) = (eval (unanno t1) p (splitEv_T_l s (get_et e)))).
+      assert (get_et (evc e0 e1) = (eval (unanno (unannoPar t1)) p (splitEv_T_l s (get_et e)))).
       {
         destruct s; destruct s.
         ++
@@ -520,7 +579,7 @@ Proof.
       rewrite H6.
       
 
-      assert (get_et (evc e2 e3) = (eval (unanno t2) p (splitEv_T_r s (get_et e)))).
+      assert (get_et (evc e2 e3) = (eval (unanno (unannoPar t2)) p (splitEv_T_r s (get_et e)))).
       {
         repeat do_pl_immut; subst.
         destruct s.
@@ -547,7 +606,7 @@ Proof.
       annogo.
       simpl in *.
       do_suffix blah.
-      do_suffix blah'.
+      (* do_suffix blah'. *)
       destruct_conjs; subst.
       repeat do_restl.
 
@@ -556,11 +615,11 @@ Proof.
       assert (e3 = get_et (evc e2 e3)) by tauto.
       jkjke.
 
-      assert (get_et (evc e0 e1) = (eval (unanno t1) p (splitEv_T_l s (get_et e)))).
+      assert (get_et (evc e0 e1) = (eval (unanno (unannoPar t)) p (splitEv_T_l s (get_et e)))).
       {
         destruct s; destruct s.
         ++
-          eapply IHt1;
+          eapply IHt;
           eassumption.
         ++
           unfold splitEv_T_l.
@@ -568,29 +627,68 @@ Proof.
           jkjke.
       }
       ff.
-      rewrite H6.
-      
+      rewrite H5.
 
-      assert (get_et (evc e2 e3) = (eval (unanno t2) p (splitEv_T_r s (get_et e)))).
+      do_pl_immut.
+      subst.
+       Lemma evc_inv: forall e,
+              e = evc (get_bits e) (get_et e).
+          Proof.
+            destruct e; eauto.
+          Defined.
+
+      assert (e3 = (eval (unanno a) p (splitEv_T_r s (get_et e)))).
       {
-        repeat do_pl_immut; subst.
-        destruct s.
-        destruct s0.
-        ++
-          unfold splitEv_T_r.
-          eauto.
-        ++
-          assert (mt = get_et (evc [] mt)) by tauto.
-          jkjke.
-          ff.
+        rewrite par_evidence in *.
+         destruct s.
+         destruct s; destruct s0;
+           simpl in *.
+         +
+           rewrite eval_aeval with (i:=0).
+           rewrite aeval_anno.
+           erewrite <- remote_Evidence_Type_Axiom. (*with (bits:=[]). *)
+           rewrite at_evidence.
+           erewrite <- evc_inv.
+           rewrite Heqe2.
+           ff.
+         +
+           rewrite eval_aeval with (i:=0).
+           rewrite aeval_anno.
+           unfold mt_evc in *.
+           erewrite <- remote_Evidence_Type_Axiom. (*with (bits:=[]). *)
+           rewrite at_evidence.
+          (* erewrite <- evc_inv. *)
+           rewrite Heqe2.
+           ff.
+         +
+           rewrite eval_aeval with (i:=0).
+           rewrite aeval_anno.
+           unfold mt_evc in *.
+           erewrite <- remote_Evidence_Type_Axiom. (*with (bits:=[]). *)
+           rewrite at_evidence.
+           erewrite <- evc_inv.
+           rewrite Heqe2.
+           ff.
+         +
+           rewrite eval_aeval with (i:=0).
+           rewrite aeval_anno.
+           unfold mt_evc in *.
+           erewrite <- remote_Evidence_Type_Axiom. (*with (bits:=[]). *)
+           rewrite at_evidence.
+          (* erewrite <- evc_inv. *)
+           rewrite Heqe2.
+           ff.
       }
-      ff.
+      rewrite H5.
+      tauto.
+      Unshelve.
+      eauto.
 Defined.
 
 Lemma cvm_refines_lts_evidence : forall t tr tr' bits bits' et et' p p',
     well_formed_r t ->
     copland_compile t (mk_st (evc bits et) tr p) = (Some tt, (mk_st (evc bits' et') tr' p')) ->
-    et' = (Term_Defs.eval (unanno t) p et).
+    et' = (Term_Defs.eval (unanno (unannoPar t)) p et).
 Proof.
   intros.
   assert (et = get_et (evc bits et)) by tauto.
@@ -599,8 +697,12 @@ Proof.
   eapply cvm_refines_lts_evidence'; eauto.
 Defined.
 
+Definition lts_remote_events (t:AnnoTerm) (p:Plc) : list Ev.
+Admitted.
+
+
 Axiom remote_LTS: forall t n et, 
-    lstar (conf t n et) (remote_events t n) (stop n (aeval t n et)).
+    lstar (conf t n et) (lts_remote_events t n) (stop n (aeval t n et)).
 
 Lemma eval_aeval: forall t1 p et,
     eval (unanno t1) p et = aeval t1 p et.
@@ -626,18 +728,111 @@ Proof.
     eauto. 
 Defined.
 
-Lemma cvm_refines_lts_event_ordering : forall t tr bits bits' et et' p p',
+Inductive cvm_to_lts_event: Ev -> CVM_Event -> Prop :=
+| cvmlts_copy: forall n p,
+    cvm_to_lts_event (copy n p) (cvm_copy n p)
+| cvmlts_umeas: forall n p i args tpl tid,
+    cvm_to_lts_event (umeas n p i args tpl tid)
+                     (cvm_umeas n p i args tpl tid)
+| cvmlts_sign: forall n p et,
+    cvm_to_lts_event (sign n p et)
+                     (cvm_sign n p et)
+| cvmlts_hash: forall n p et,
+    cvm_to_lts_event (hash n p et)
+                     (cvm_hash n p et)
+| cvmlts_req: forall n p q t et,
+    cvm_to_lts_event (req n p q t et)
+                     (cvm_req n p q t et)
+| cvmlts_rpy: forall n p q et,
+    cvm_to_lts_event (rpy n p q et)
+                     (cvm_rpy n p q et)
+| cvm_split: forall n p,
+    cvm_to_lts_event (Term_Defs.split n p)
+                     (cvm_split n p)
+| cvmlts_join: forall n p,
+    cvm_to_lts_event (Term_Defs.join n p)
+                     (cvm_join n p)
+| cvmlts_splitp: forall n p loc t et,
+    cvm_to_lts_event (Term_Defs.split n p)
+                     (cvm_splitp n loc p t et)
+| cvmlts_joinp: forall n p loc t,
+    cvm_to_lts_event (Term_Defs.join n p)
+                     (cvm_joinp n loc p t).
+Hint Constructors cvm_to_lts_event : core.
+
+Check shuffled_events.
+Locate shuffled_events.
+Locate shuffle.
+
+
+Inductive cvm_to_lts_trace: list Ev -> list CVM_Event -> Prop :=
+| cvm_shuffle: forall l1 cvm_l1 n n0 loc p t et,
+    cvm_to_lts_trace l1 cvm_l1 ->
+    cvm_to_lts_trace
+      ([Term_Defs.split n p] ++
+       (shuffled_events l1 (lts_remote_events t p)) ++
+       [Term_Defs.join n0 p])
+      ([cvm_splitp n loc p t et] ++ cvm_l1 ++ [cvm_joinp n0 loc p t])
+| cvm_move: forall tr_lts tr_cvm rest_lts rest_cvm,
+    cvm_to_lts_trace tr_lts tr_cvm ->
+    cvm_to_lts_trace
+      rest_lts
+      rest_cvm ->
+    cvm_to_lts_trace (tr_lts ++ rest_lts) (tr_cvm ++ rest_cvm)
+| cvm_move_one: forall e1_lts e1_cvm (*rest_lts rest_cvm*),
+    cvm_to_lts_event e1_lts e1_cvm ->
+    cvm_to_lts_trace
+      ([e1_lts] (* ++ rest_lts *))
+      ([e1_cvm] (* ++ rest_cvm *)).
+Hint Constructors cvm_to_lts_trace : core.
+
+Lemma cvm_refines_lts_event_ordering : forall t cvm_tr bits bits' et et' p p',
     well_formed_r t ->
     (*Ev_Shape e et -> *)
-    copland_compile t (mk_st (evc bits et) [] p) = (Some tt, (mk_st (evc bits' et') tr p')) ->
-    lstar (conf t p et) tr (stop p (aeval t p et)).
+    copland_compile t (mk_st (evc bits et) [] p) = (Some tt, (mk_st (evc bits' et') cvm_tr p')) ->
+    exists tr,
+    lstar (conf (unannoPar t) p et) tr (stop p (aeval (unannoPar t) p et)) /\
+    cvm_to_lts_trace tr cvm_tr.
 Proof.
-  intros t tr bits bits' et et' p p' H H'.
+  intros t cvm_tr bits bits' et et' p p' H.
   generalizeEverythingElse t.
   induction t; intros.
   - (* aasp case *)
     destruct a;
       df;
+      eexists;
+      split;
+      econstructor; try econstructor.
+    
+
+
+
+    (*
+    +
+      invc H'';
+        try solve_by_inversion.
+      invc H0;
+        try solve_by_inversion.
+      invc H1; try solve_by_inversion.
+    +
+      invc H'';
+        try solve_by_inversion.
+      invc H0;
+        try solve_by_inversion.
+      invc H1; try solve_by_inversion.
+    +
+      invc H'';
+        try solve_by_inversion.
+      invc H0;
+        try solve_by_inversion.
+      invc H1; try solve_by_inversion.
+    +
+      invc H'';
+        try solve_by_inversion.
+      invc H0;
+        try solve_by_inversion.
+      invc H1; try solve_by_inversion.
+    (*
       econstructor; try (econstructor; reflexivity).
 
   (*
@@ -650,14 +845,19 @@ Proof.
       }
       rewrite <- H0.
       econstructor; try (econstructor; reflexivity). *)
+     *)
+     *)
+    
+      
     
     
   - (* aatt case *)
     destruct r.
     repeat (df; try dohtac; df).
     
-    assert (lstar (conf t n et) (remote_events t n) (stop n (aeval t n et))).
+    assert (lstar (conf a n et) (lts_remote_events a n) (stop n (aeval a n et))).
     {
+      
       apply remote_LTS.
     }
 
@@ -676,6 +876,101 @@ Proof.
       eassumption.
     }
     rewrite H1. *)
+
+
+
+
+    (*
+
+    invc H''; try solve_by_inversion.
+    invc H2; try solve_by_inversion.
+
+    assert ((req n0 p' n (unanno a) et :: tr0) =
+            [req n0 p' n (unanno a) et] ++ tr0).
+    admit.
+    rewrite H2; clear H2.
+
+    assert (    (cvm_req n0 p' n (unanno a) et
+     :: remote_events a n ++
+     [cvm_rpy (Nat.pred n1) p' n (get_et (toRemote a n (evc bits et)))]) =
+                ( [cvm_req n0 p' n (unanno a) et]
+     ++ remote_events a n ++
+     [cvm_rpy (Nat.pred n1) p' n (get_et (toRemote a n (evc bits et)))])).
+    admit.
+    rewrite H2; clear H2.
+    econstructor.
+    econstructor.
+    econstructor.
+    simpl in *.
+
+    Lemma lstar_at_decomp: forall i p a n et tr,
+      lstar (rem i p (conf a n et)) tr (stop p (aeval a n et)) ->
+      exists tr1, 
+        tr = tr1 ++ [rpy (Nat.pred i) p n (aeval a n et)] /\
+        lstar (conf a n et) tr1 (stop n (aeval a n et)).
+    Proof.
+    Admitted.
+
+    edestruct lstar_at_decomp; eauto.
+    destruct_conjs.
+    rewrite H2.
+
+    econstructor.
+
+    Axiom remote_lts_axiom: forall a n et x,
+      lstar (conf a n et) x (stop n (aeval a n et)) ->
+      x = lts_remote_events a n.
+
+    simpl.
+
+    assert (x = lts_remote_events a n).
+    {
+      eapply remote_lts_axiom; eauto.
+    }
+    rewrite H5.
+
+    admit. (* TODO: lemma or extra rule in relation? *)
+    econstructor.
+    rewrite remote_Evidence_Type_Axiom.
+    econstructor.
+    
+
+    (*
+    erewrite remote_lts_axiom.
+    
+    
+
+    simpl in *.
+
+    Check lstar_strem.
+
+    invc H3; try solve_by_inversion.
+    admit.
+    invc H2.
+    invc H2; try solve_by_inversion.
+    admit.
+    invc H2.
+    invc H9
+    invc H4; try solve_by_inversion.
+    invc H2; try solve_by_inversion.
+
+
+    
+    eapply cvm_move.
+*)
+
+
+
+     *)
+
+
+
+
+    eexists.
+    split.
+    
+
+    
     
 
     eapply lstar_tran.
@@ -686,9 +981,10 @@ Proof.
     cbn.
     
     apply H0.
+    (*
     jkjke.
-    ff.
-    assert (et' = (aeval t n et)).
+    ff. *)
+    assert (et' = (aeval a n et)).
     {
       erewrite <- remote_Evidence_Type_Axiom.
       jkjke.
@@ -700,26 +996,84 @@ Proof.
     econstructor.
     apply stattstop.
     econstructor.
+    simpl.
+
+     assert ((req n0 p' n (unanno a) et  :: lts_remote_events a n ++ [rpy (Nat.pred n1) p' n (aeval a n et)]) =
+            [req n0 p' n (unanno a) et] ++  lts_remote_events a n ++ [rpy (Nat.pred n1) p' n (aeval a n et)]).
+    admit.
+    rewrite H1; clear H1.
+
+    assert (    (cvm_req n0 p' n (unanno a) et
+     :: remote_events a n ++
+     [cvm_rpy (Nat.pred n1) p' n (get_et (toRemote a n (evc bits et)))]) =
+                ( [cvm_req n0 p' n (unanno a) et]
+     ++ remote_events a n ++
+     [cvm_rpy (Nat.pred n1) p' n (get_et (toRemote a n (evc bits et)))])).
+    admit.
+    rewrite H1; clear H1.
+    econstructor.
+    econstructor.
+    econstructor.
+
+    econstructor.
+
+    admit. (* TODO: lemma or extra rule in relation? *)
+    econstructor.
+    rewrite remote_Evidence_Type_Axiom.
+    econstructor.
+    
+
+    
+    
   -  
     do_wf_pieces.
     edestruct alseq_decomp; eauto.
     destruct_conjs.
     destruct x.
-    econstructor.
-    econstructor.
     subst.
-    eapply lstar_transitive.
+    df.
+    edestruct IHt1; eauto.
+    edestruct IHt2; eauto.
+    destruct_conjs.
+    eexists.
+    split.
+    +
+      
+
+      eapply lstar_transitive.
+      eapply lstar_silent_tran.
+      econstructor.
+
     eapply lstar_stls.
     df.
+    simpl.
+    eassumption.
+    (*
     eapply IHt1.
     eassumption.
-    eassumption.
+    eassumption. *)
 
     eapply lstar_silent_tran.
     apply stlseqstop.
     df.
     repeat do_pl_immut.
-    subst.   
+    subst.
+
+    assert (e0 = Term_Defs.eval (unanno (unannoPar t1)) p et).
+    eapply cvm_refines_lts_evidence; eauto.
+    subst.
+    rewrite <- eval_aeval.
+    
+
+    
+    eassumption.
+    +
+      econstructor.
+      eauto.
+      eauto.
+
+
+    (*
     eapply IHt2. (*with (e:= x). *)
     eassumption.
     assert (e0 = Term_Defs.eval (unanno t1) p et).
@@ -729,6 +1083,8 @@ Proof.
     rewrite <- eval_aeval.
     
     eassumption.
+     *)
+    
     
   -    (* abseq case *)
     do_wf_pieces.
@@ -738,6 +1094,7 @@ Proof.
       vmsts.
       dosome.
       df.
+      simpl.
 
       do_suffix blah.
       do_suffix blah'.
@@ -747,6 +1104,13 @@ Proof.
       repeat do_pl_immut.
       subst.
       repeat rewrite <- app_assoc.
+      edestruct IHt1; eauto.
+      edestruct IHt2; eauto.
+      destruct_conjs.
+
+      eexists.
+      split.
+      ++
 
       eapply lstar_tran.
       econstructor.
@@ -755,16 +1119,21 @@ Proof.
       eapply lstar_transitive.
       simpl.
 
-      eapply lstar_stbsl.  
+      eapply lstar_stbsl.
+      eassumption.
+
+      (*
       
       eapply IHt1.
-      eassumption.
+      eassumption. 
       (*
     
     2: {
       eassumption.
       } *)
       eassumption.
+       *)
+      
       
       unfold run_cvm in *.
       monad_unfold.
@@ -774,6 +1143,10 @@ Proof.
       
       eapply lstar_transitive.
       eapply lstar_stbsr.
+
+      eassumption.
+
+      (*
       
       eapply IHt2.
       eassumption.
@@ -781,14 +1154,294 @@ Proof.
     2: {
       eassumption.
       } *)
-      eassumption.
+      eassumption. *)
       
       econstructor.
 
       eapply stbsrstop.
       econstructor.
+      ++
+        simpl.
+        assert ((Term_Defs.split n p :: x ++ x0 ++ [join (Nat.pred n0) p]) =
+                ([Term_Defs.split n p] ++ x ++ x0 ++ [join (Nat.pred n0) p])).
+        admit.
+        rewrite H8.
 
+        assert ((StVM.cvm_split n p :: blah' ++ blah ++ [cvm_join (Nat.pred n0) p]) =
+                ([StVM.cvm_split n p] ++ blah' ++ blah ++ [cvm_join (Nat.pred n0) p])).
+        admit.
+        rewrite H9.
+        eauto.
+        econstructor.
+        econstructor.
+        econstructor.
+        eauto.
+    +
+      
+              df.
+      vmsts.
+      dosome.
+      df.
+      simpl.
 
+      do_suffix blah.
+      do_suffix blah'.
+      destruct_conjs; subst.
+      repeat do_restl.
+      
+      repeat do_pl_immut.
+      subst.
+      repeat rewrite <- app_assoc.
+      edestruct IHt1; eauto.
+      edestruct IHt2; eauto.
+      destruct_conjs.
+
+      eexists.
+      split.
+      ++
+
+      eapply lstar_tran.
+      econstructor.
+      simpl.
+
+      eapply lstar_transitive.
+      simpl.
+
+      eapply lstar_stbsl.
+      eassumption.
+
+      (*
+      
+      eapply IHt1.
+      eassumption. 
+      (*
+    
+    2: {
+      eassumption.
+      } *)
+      eassumption.
+       *)
+      
+      
+      unfold run_cvm in *.
+      monad_unfold.
+
+      eapply lstar_silent_tran.
+      apply stbslstop.
+      
+      eapply lstar_transitive.
+      eapply lstar_stbsr.
+
+      eassumption.
+
+      (*
+      
+      eapply IHt2.
+      eassumption.
+      (*
+    2: {
+      eassumption.
+      } *)
+      eassumption. *)
+      
+      econstructor.
+
+      eapply stbsrstop.
+      econstructor.
+      ++
+        simpl.
+        assert ((Term_Defs.split n p :: x ++ x0 ++ [join (Nat.pred n0) p]) =
+                ([Term_Defs.split n p] ++ x ++ x0 ++ [join (Nat.pred n0) p])).
+        admit.
+        rewrite H8.
+
+        assert ((StVM.cvm_split n p :: blah' ++ blah ++ [cvm_join (Nat.pred n0) p]) =
+                ([StVM.cvm_split n p] ++ blah' ++ blah ++ [cvm_join (Nat.pred n0) p])).
+        admit.
+        rewrite H9.
+        eauto.
+        econstructor.
+        econstructor.
+        econstructor.
+        eauto.
+    +
+            df.
+      vmsts.
+      dosome.
+      df.
+      simpl.
+
+      do_suffix blah.
+      do_suffix blah'.
+      destruct_conjs; subst.
+      repeat do_restl.
+      
+      repeat do_pl_immut.
+      subst.
+      repeat rewrite <- app_assoc.
+      edestruct IHt1; eauto.
+      edestruct IHt2; eauto.
+      destruct_conjs.
+
+      eexists.
+      split.
+      ++
+
+      eapply lstar_tran.
+      econstructor.
+      simpl.
+
+      eapply lstar_transitive.
+      simpl.
+
+      eapply lstar_stbsl.
+      eassumption.
+
+      (*
+      
+      eapply IHt1.
+      eassumption. 
+      (*
+    
+    2: {
+      eassumption.
+      } *)
+      eassumption.
+       *)
+      
+      
+      unfold run_cvm in *.
+      monad_unfold.
+
+      eapply lstar_silent_tran.
+      apply stbslstop.
+      
+      eapply lstar_transitive.
+      eapply lstar_stbsr.
+
+      eassumption.
+
+      (*
+      
+      eapply IHt2.
+      eassumption.
+      (*
+    2: {
+      eassumption.
+      } *)
+      eassumption. *)
+      
+      econstructor.
+
+      eapply stbsrstop.
+      econstructor.
+      ++
+        simpl.
+        assert ((Term_Defs.split n p :: x ++ x0 ++ [join (Nat.pred n0) p]) =
+                ([Term_Defs.split n p] ++ x ++ x0 ++ [join (Nat.pred n0) p])).
+        admit.
+        rewrite H8.
+
+        assert ((StVM.cvm_split n p :: blah' ++ blah ++ [cvm_join (Nat.pred n0) p]) =
+                ([StVM.cvm_split n p] ++ blah' ++ blah ++ [cvm_join (Nat.pred n0) p])).
+        admit.
+        rewrite H9.
+        eauto.
+        econstructor.
+        econstructor.
+        econstructor.
+        eauto.
+    +
+            df.
+      vmsts.
+      dosome.
+      df.
+      simpl.
+
+      do_suffix blah.
+      do_suffix blah'.
+      destruct_conjs; subst.
+      repeat do_restl.
+      
+      repeat do_pl_immut.
+      subst.
+      repeat rewrite <- app_assoc.
+      edestruct IHt1; eauto.
+      edestruct IHt2; eauto.
+      destruct_conjs.
+
+      eexists.
+      split.
+      ++
+
+      eapply lstar_tran.
+      econstructor.
+      simpl.
+
+      eapply lstar_transitive.
+      simpl.
+
+      eapply lstar_stbsl.
+      eassumption.
+
+      (*
+      
+      eapply IHt1.
+      eassumption. 
+      (*
+    
+    2: {
+      eassumption.
+      } *)
+      eassumption.
+       *)
+      
+      
+      unfold run_cvm in *.
+      monad_unfold.
+
+      eapply lstar_silent_tran.
+      apply stbslstop.
+      
+      eapply lstar_transitive.
+      eapply lstar_stbsr.
+
+      eassumption.
+
+      (*
+      
+      eapply IHt2.
+      eassumption.
+      (*
+    2: {
+      eassumption.
+      } *)
+      eassumption. *)
+      
+      econstructor.
+
+      eapply stbsrstop.
+      econstructor.
+      ++
+        simpl.
+        assert ((Term_Defs.split n p :: x ++ x0 ++ [join (Nat.pred n0) p]) =
+                ([Term_Defs.split n p] ++ x ++ x0 ++ [join (Nat.pred n0) p])).
+        admit.
+        rewrite H8.
+
+        assert ((StVM.cvm_split n p :: blah' ++ blah ++ [cvm_join (Nat.pred n0) p]) =
+                ([StVM.cvm_split n p] ++ blah' ++ blah ++ [cvm_join (Nat.pred n0) p])).
+        admit.
+        rewrite H9.
+        eauto.
+        econstructor.
+        econstructor.
+        econstructor.
+        eauto.
+
+        
+    
+(*   
     +
       df.
       vmsts.
@@ -951,10 +1604,493 @@ Proof.
 
       eapply stbsrstop.
       econstructor.
+ *)
+
+        Axiom par_events : forall t p,
+    parallel_vm_events t p = remote_trace t p.
+
+      Axiom bpar_shuffle : forall x tr p t1 t2 et1 et2,
+          lstar (conf t1 p et1) tr (stop p (aeval t1 p et1)) ->
+    lstar (bp x (conf t1 p et1) (conf t2 p et2))
+          (shuffled_events tr
+                           (lts_remote_events t2 p))
+          (bp x (stop p (aeval t1 p et1)) (stop p (aeval t2 p et2))).
 
   - (* abpar case *)
     do_wf_pieces.
     destruct r; destruct s; destruct s; destruct s0.
+    +
+      df.
+      vmsts.
+      dosome.
+      df.
+      simpl.
+
+      do_suffix blah.
+      (* do_suffix blah'. *)
+      destruct_conjs; subst.
+      repeat do_restl.
+      
+      repeat do_pl_immut.
+      subst.
+      repeat rewrite <- app_assoc.
+      edestruct IHt; eauto.
+      (*
+      edestruct IHt2; eauto. *)
+      destruct_conjs.
+
+      Check lts_remote_events.
+
+
+      exists ([Term_Defs.split n p] ++ (shuffled_events x (lts_remote_events a p)) ++
+                               [Term_Defs.join (Nat.pred n0) p]).
+
+      
+      split.
+      ++
+
+      eapply lstar_tran.
+      econstructor.
+      simpl.
+
+      eapply lstar_transitive.
+      simpl.
+
+
+
+      simpl.
+      apply bpar_shuffle.
+      eassumption.
+
+
+
+      (*
+
+      eapply lstar_stbparl.
+      eassumption.
+
+      (*
+      
+      eapply IHt1.
+      eassumption. 
+      (*
+    
+    2: {
+      eassumption.
+      } *)
+      eassumption.
+       *)
+      
+      
+      unfold run_cvm in *.
+      monad_unfold.
+
+      (*
+
+      eapply lstar_silent_tran.
+      apply stbplstop. *)
+      
+      eapply lstar_transitive.
+      eapply lstar_stbparr.
+
+      apply remote_LTS.  *)
+      econstructor.
+      eapply stbpstop.
+      econstructor.
+      ++
+
+        (*
+        simpl.
+
+        assert ( (Term_Defs.split n p :: x ++ lts_remote_events a p ++ [join (Nat.pred n0) p]) =
+                 ([Term_Defs.split n p] ++ x ++ lts_remote_events a p ++ [join (Nat.pred n0) p])).
+        admit.
+        rewrite H5; clear H5.
+
+
+
+        assert ((cvm_splitp n l p a et :: blah ++ [cvm_joinp (Nat.pred n0) l p a]) =
+                ([cvm_splitp n l p a et] ++ blah ++ [cvm_joinp (Nat.pred n0) l p a])).
+        admit.
+        rewrite H5; clear H5. *)
+
+        eapply cvm_shuffle.
+        eassumption.
+    +
+            df.
+      vmsts.
+      dosome.
+      df.
+      simpl.
+
+      do_suffix blah.
+      (* do_suffix blah'. *)
+      destruct_conjs; subst.
+      repeat do_restl.
+      
+      repeat do_pl_immut.
+      subst.
+      repeat rewrite <- app_assoc.
+      edestruct IHt; eauto.
+      (*
+      edestruct IHt2; eauto. *)
+      destruct_conjs.
+
+      Check lts_remote_events.
+
+
+      exists ([Term_Defs.split n p] ++ (shuffled_events x (lts_remote_events a p)) ++
+                               [Term_Defs.join (Nat.pred n0) p]).
+
+      
+      split.
+      ++
+
+      eapply lstar_tran.
+      econstructor.
+      simpl.
+
+      eapply lstar_transitive.
+      simpl.
+
+
+
+      simpl.
+      apply bpar_shuffle.
+      eassumption.
+
+
+
+      (*
+
+      eapply lstar_stbparl.
+      eassumption.
+
+      (*
+      
+      eapply IHt1.
+      eassumption. 
+      (*
+    
+    2: {
+      eassumption.
+      } *)
+      eassumption.
+       *)
+      
+      
+      unfold run_cvm in *.
+      monad_unfold.
+
+      (*
+
+      eapply lstar_silent_tran.
+      apply stbplstop. *)
+      
+      eapply lstar_transitive.
+      eapply lstar_stbparr.
+
+      apply remote_LTS.  *)
+      econstructor.
+      eapply stbpstop.
+      econstructor.
+      ++
+
+        (*
+        simpl.
+
+        assert ( (Term_Defs.split n p :: x ++ lts_remote_events a p ++ [join (Nat.pred n0) p]) =
+                 ([Term_Defs.split n p] ++ x ++ lts_remote_events a p ++ [join (Nat.pred n0) p])).
+        admit.
+        rewrite H5; clear H5.
+
+
+
+        assert ((cvm_splitp n l p a et :: blah ++ [cvm_joinp (Nat.pred n0) l p a]) =
+                ([cvm_splitp n l p a et] ++ blah ++ [cvm_joinp (Nat.pred n0) l p a])).
+        admit.
+        rewrite H5; clear H5. *)
+
+        eapply cvm_shuffle.
+        eassumption.
+    +
+            df.
+      vmsts.
+      dosome.
+      df.
+      simpl.
+
+      do_suffix blah.
+      (* do_suffix blah'. *)
+      destruct_conjs; subst.
+      repeat do_restl.
+      
+      repeat do_pl_immut.
+      subst.
+      repeat rewrite <- app_assoc.
+      edestruct IHt; eauto.
+      (*
+      edestruct IHt2; eauto. *)
+      destruct_conjs.
+
+      Check lts_remote_events.
+
+
+      exists ([Term_Defs.split n p] ++ (shuffled_events x (lts_remote_events a p)) ++
+                               [Term_Defs.join (Nat.pred n0) p]).
+
+      
+      split.
+      ++
+
+      eapply lstar_tran.
+      econstructor.
+      simpl.
+
+      eapply lstar_transitive.
+      simpl.
+
+
+
+      simpl.
+      apply bpar_shuffle.
+      eassumption.
+
+
+
+      (*
+
+      eapply lstar_stbparl.
+      eassumption.
+
+      (*
+      
+      eapply IHt1.
+      eassumption. 
+      (*
+    
+    2: {
+      eassumption.
+      } *)
+      eassumption.
+       *)
+      
+      
+      unfold run_cvm in *.
+      monad_unfold.
+
+      (*
+
+      eapply lstar_silent_tran.
+      apply stbplstop. *)
+      
+      eapply lstar_transitive.
+      eapply lstar_stbparr.
+
+      apply remote_LTS.  *)
+      econstructor.
+      eapply stbpstop.
+      econstructor.
+      ++
+
+        (*
+        simpl.
+
+        assert ( (Term_Defs.split n p :: x ++ lts_remote_events a p ++ [join (Nat.pred n0) p]) =
+                 ([Term_Defs.split n p] ++ x ++ lts_remote_events a p ++ [join (Nat.pred n0) p])).
+        admit.
+        rewrite H5; clear H5.
+
+
+
+        assert ((cvm_splitp n l p a et :: blah ++ [cvm_joinp (Nat.pred n0) l p a]) =
+                ([cvm_splitp n l p a et] ++ blah ++ [cvm_joinp (Nat.pred n0) l p a])).
+        admit.
+        rewrite H5; clear H5. *)
+
+        eapply cvm_shuffle.
+        eassumption.
+    +
+            df.
+      vmsts.
+      dosome.
+      df.
+      simpl.
+
+      do_suffix blah.
+      (* do_suffix blah'. *)
+      destruct_conjs; subst.
+      repeat do_restl.
+      
+      repeat do_pl_immut.
+      subst.
+      repeat rewrite <- app_assoc.
+      edestruct IHt; eauto.
+      (*
+      edestruct IHt2; eauto. *)
+      destruct_conjs.
+
+      Check lts_remote_events.
+
+
+      exists ([Term_Defs.split n p] ++ (shuffled_events x (lts_remote_events a p)) ++
+                               [Term_Defs.join (Nat.pred n0) p]).
+
+      
+      split.
+      ++
+
+      eapply lstar_tran.
+      econstructor.
+      simpl.
+
+      eapply lstar_transitive.
+      simpl.
+
+
+
+      simpl.
+      apply bpar_shuffle.
+      eassumption.
+
+
+
+      (*
+
+      eapply lstar_stbparl.
+      eassumption.
+
+      (*
+      
+      eapply IHt1.
+      eassumption. 
+      (*
+    
+    2: {
+      eassumption.
+      } *)
+      eassumption.
+       *)
+      
+      
+      unfold run_cvm in *.
+      monad_unfold.
+
+      (*
+
+      eapply lstar_silent_tran.
+      apply stbplstop. *)
+      
+      eapply lstar_transitive.
+      eapply lstar_stbparr.
+
+      apply remote_LTS.  *)
+      econstructor.
+      eapply stbpstop.
+      econstructor.
+      ++
+
+        (*
+        simpl.
+
+        assert ( (Term_Defs.split n p :: x ++ lts_remote_events a p ++ [join (Nat.pred n0) p]) =
+                 ([Term_Defs.split n p] ++ x ++ lts_remote_events a p ++ [join (Nat.pred n0) p])).
+        admit.
+        rewrite H5; clear H5.
+
+
+
+        assert ((cvm_splitp n l p a et :: blah ++ [cvm_joinp (Nat.pred n0) l p a]) =
+                ([cvm_splitp n l p a et] ++ blah ++ [cvm_joinp (Nat.pred n0) l p a])).
+        admit.
+        rewrite H5; clear H5. *)
+
+        eapply cvm_shuffle.
+        eassumption.
+
+        
+
+
+
+
+
+
+
+
+(****  OLD CVM REFINES LTS ORDERING PROOF   
+
+
+
+
+
+
+
+
+        
+
+
+
+
+      
+        econstructor.
+        econstructor.
+        econstructor.
+        econstructor
+
+
+
+
+
+
+        
+        
+
+      eapply lts_remote_events.
+
+      
+
+      eassumption.
+
+      (*
+      
+      eapply IHt2.
+      eassumption.
+      (*
+    2: {
+      eassumption.
+      } *)
+      eassumption. *)
+      
+      econstructor.
+
+      eapply stbsrstop.
+      econstructor.
+      ++
+        simpl.
+        assert ((Term_Defs.split n p :: x ++ x0 ++ [join (Nat.pred n0) p]) =
+                ([Term_Defs.split n p] ++ x ++ x0 ++ [join (Nat.pred n0) p])).
+        admit.
+        rewrite H8.
+
+        assert ((StVM.cvm_split n p :: blah' ++ blah ++ [cvm_join (Nat.pred n0) p]) =
+                ([StVM.cvm_split n p] ++ blah' ++ blah ++ [cvm_join (Nat.pred n0) p])).
+        admit.
+        rewrite H9.
+        eauto.
+        econstructor.
+        econstructor.
+        econstructor.
+        eauto.
+
+
+
+
+
+
+
+
+
+    
     +
       df.
       vmsts.
@@ -1183,6 +2319,7 @@ Proof.
       eapply stbpstop.
       econstructor.
 Defined.
+*)
 
 Lemma cvm_refines_lts_event_ordering_corrolary : forall t tr bits bits' et et' p p',
     well_formed_r t ->
